theories/Data/Monads/OptionMonad.v
@@ -6,7 +6,7 @@ Set Strict Implicit.
 Import MonadNotation.
 Local Open Scope monad_scope.
 
-Global Instance Monad_option : Monad option :=
+Polymorphic Global Instance Monad_option : Monad option :=
 { ret  := @Some
 ; bind := fun _ _ c1 c2 => match c1 with
                              | None => None
@@ -14,10 +14,10 @@ Global Instance Monad_option : Monad option :=
                            end
 }.
 
-Global Instance Zero_option : MonadZero option :=
+Polymorphic Global Instance Zero_option : MonadZero option :=
 { mzero := @None }.
 
-Global Instance Plus_option : MonadPlus option :=
+Polymorphic Global Instance Plus_option : MonadPlus option :=
 { mplus _A _B aM bM :=
     match aM with
     | None => liftM inr bM
@@ -34,11 +34,12 @@ Global Instance Exception_option : MonadExc unit option :=
 }.
 
 Section Trans.
-  Variable m : Type -> Type.
+  Universe i j.
+  Variable m : Type@{i} -> Type@{j}.
 
   Inductive optionT a := mkOptionT { unOptionT : m (option a) }.
 
-  Context {M : Monad m}.
+  Context {M : Monad@{i j} m}.
 
   Global Instance Monad_optionT : Monad optionT :=
   { ret _A := fun x => mkOptionT (ret (Some x))
@@ -53,15 +54,15 @@ Section Trans.
   Global Instance Zero_optionT : MonadZero optionT :=
   { mzero _A := mkOptionT (ret None) }.
 
-  Global Instance MonadT_optionT : MonadT optionT m :=
+  Polymorphic Global Instance MonadT_optionT : MonadT optionT m :=
   { lift _A aM := mkOptionT (liftM ret aM) }.
 
-  Global Instance State_optionT {T} (SM : MonadState T m) : MonadState T optionT :=
+  Polymorphic Global Instance State_optionT {T} (SM : MonadState T m) : MonadState T optionT :=
   { get := lift get
   ; put v := lift (put v)
   }.
 
-  Instance Plus_optionT_right : MonadPlus optionT :=
+  Polymorphic Instance Plus_optionT_right : MonadPlus optionT :=
   { mplus _A _B a b :=
       mkOptionT (bind (unOptionT b) (fun b =>
         match b with
@@ -75,7 +76,7 @@ Section Trans.
         end))
   }.
 
-  Instance Plus_optionT_left : MonadPlus optionT :=
+  Polymorphic Instance Plus_optionT_left : MonadPlus optionT :=
   { mplus _A _B a b :=
       mkOptionT (bind (unOptionT a) (fun a =>
         match a with
@@ -89,14 +90,14 @@ Section Trans.
         end))
   }.
 
-  Global Instance Plus_optionT : MonadPlus optionT := Plus_optionT_left.
+  Polymorphic Global Instance Plus_optionT : MonadPlus optionT := Plus_optionT_left.
 
-  Global Instance Reader_optionT {T} (SM : MonadReader T m) : MonadReader T optionT :=
+  Polymorphic Global Instance Reader_optionT {T} (SM : MonadReader T m) : MonadReader T optionT :=
   { ask := lift ask
   ; local _T v cmd := mkOptionT (local v (unOptionT cmd))
   }.
 
-  Instance OptionTError : MonadExc unit optionT :=
+  Polymorphic Global Instance OptionTErros : MonadExc unit optionT :=
   { raise _u _A := mzero
   ; catch _A aMM f := mkOptionT
       (aM <- unOptionT aMM ;;
